Lab3a

statdb-cli/extract/Nat.hs
@@ -1,5 +1,0 @@
-{-# OPTIONS_GHC -F -pgmF ./fiximports.py #-}
-module Nat where
-
-import qualified Prelude
-
