statdb-cli/extract/StatDbAPI.hs
@@ -1,7 +1,0 @@
-{-# OPTIONS_GHC -F -pgmF ./fiximports.py #-}
-module StatDbAPI where
-
-import qualified Prelude
-
-type State = ([]) Prelude.Integer
-
