src/Lab2/RemappedDiskImpl.v
@@ -15,10 +15,20 @@ Module RemappedDisk (bd : BadBlockAPI) <: OneDiskAPI.
       Ret r
     else
       r <- bd.read a;
-    Ret r.
+      Ret r.
 
   Definition write (a : addr) (b : block) : proc unit :=
-    Ret tt.
+    bs <- bd.getBadBlock;
+    len <- bd.size;
+    if a == bs then
+      _ <- bd.write (len-1) b;
+      Ret tt
+    else
+      if a == (len-1) then
+        Ret tt
+      else
+        _ <- bd.write a b;
+        Ret tt.
 
   Definition size : proc nat :=
     len <- bd.size;
@@ -40,21 +50,20 @@ Module RemappedDisk (bd : BadBlockAPI) <: OneDiskAPI.
   Definition recover: proc unit :=
     bd.recover.
 
-
   Inductive remapped_abstraction (bs_state : BadBlockAPI.State) (rd_disk : OneDiskAPI.State) : Prop :=
     | RemappedAbstraction :
       let bs_disk := stateDisk bs_state in
       let bs_addr := stateBadBlock bs_state in
       forall
         (* Fill in the rest of your abstraction here. *)
-        (* To refer to the contents of disk [d] at address [a], you can write [diskGet a] *)
+        (* To refer to the contents of disk [d] at address [a], you can write [diskGet d a] *) (* <-- TODO this was wrong*)
         (* To refer to the size of disk [d], you can write [diskSize d] *)
         (* You can try to prove [read_ok] to discover what you need from this abstraction *)
 
         (* Hint 1: What should be true about the non-bad blocks?   Replace [True] with what needs to be true *)
-        (Hgoodblocks : True)
+        (Hgoodblocks : forall a : nat, (a < diskSize rd_disk /\ not(a = bs_addr)) -> diskGet bs_disk a = diskGet rd_disk a)
         (* Hint 2: What should be true about the bad block? *)
-        (Hbadblock : True)
+        (Hbadblock : (bs_addr < diskSize rd_disk) -> diskGet rd_disk bs_addr = diskGet bs_disk (diskSize bs_disk - 1))
 
         (* when writing the above,  *)
         (* Hint 3: What if the bad block address is the last address? *)
@@ -75,27 +84,61 @@ Module RemappedDisk (bd : BadBlockAPI) <: OneDiskAPI.
     remapped_abstraction (BadBlockAPI.mkState [block1;block0;block0] 0 Hinbounds) [block0;block0].
   Proof.
     constructor; auto.
-    Admitted.
+    simpl. intros.
+    assert (a = 1).
+    {
+      lia.
+    }
+    intuition.
+  Qed.
 
   Example abst_2_ok : forall Hinbounds,
     remapped_abstraction (BadBlockAPI.mkState [block1;block0] 0 Hinbounds) [block0].
   Proof.
     constructor; auto.
-    Admitted.
+    simpl. intros.
+    absurd (a < 1 /\ a <> 0).
+    + lia.
+    + apply H.
+  Qed.
 
   Example abst_3_ok : forall Hinbounds,
     remapped_abstraction (BadBlockAPI.mkState [block0;block0] 1 Hinbounds) [block0].
   Proof.
     constructor; auto.
-    Admitted.
+    - simpl. intuition.
+      assert (a = 0).
+      {
+        lia.
+      }
+      intuition.
+    - simpl. intuition. absurd (1 < 1).
+      + lia.
+      + apply H.
+  Qed.
+
+  (*Unset Printing Notations.*)
+
+  Lemma some_eq : forall a b : block, Some a = Some b -> a = b.
+  Proof.
+    intros.
+    injection H. trivial.
+  Qed.
 
   Example abst_4_nok : forall Hinbounds,
     ~ remapped_abstraction (BadBlockAPI.mkState [block0;block0] 1 Hinbounds) [block1].
   Proof.
     intros.
     intro.
-    inversion H; simpl in *.
-    Admitted.
+    inversion H. simpl in *.
+    specialize (Hgoodblocks 0).
+    unfold bs_addr in Hgoodblocks.
+    simpl in Hgoodblocks. intuition.
+    apply some_eq in Hgoodblocks.
+    apply bytes_differ in Hgoodblocks.
+    { contradiction. }
+    unfold blockbytes. lia.
+  Qed.
 
   Example abst_5_nok : forall Hinbounds,
     ~ remapped_abstraction (BadBlockAPI.mkState [block1;block1] 0 Hinbounds) [block0].
@@ -103,7 +146,14 @@ Module RemappedDisk (bd : BadBlockAPI) <: OneDiskAPI.
     intros.
     intro.
     inversion H; simpl in *.
-    Admitted.
+    unfold bs_addr in Hbadblock.
+    intuition.
+    apply some_eq in Hbadblock.
+    apply bytes_differ in Hbadblock.
+    { contradiction. }
+    unfold blockbytes.
+    simpl. lia.
+  Qed.
 
   (* Due to how remapped_abstraction is defined (as an inductive), it cannot be
   unfolded. This tactic identifies abstraction relations in the hypotheses and
@@ -113,27 +163,113 @@ Module RemappedDisk (bd : BadBlockAPI) <: OneDiskAPI.
     | H : remapped_abstraction _ _ |- _ => inversion H; clear H; subst; subst_var
     end.
 
+
   Theorem init_ok : init_abstraction init recover abstr inited_any.
   Proof.
     eapply then_init_compose; eauto.
     step_proc.
-  Admitted.
+    destruct r as [| n].
+    { simpl. step_proc. }
+    simpl.
+    step_proc.
+    destruct (lt_dec r (S n)).
+    {
+      simpl. step_proc.
+      exists (let bs_disk := stateDisk state in
+         let bs_addr := stateBadBlock state in
+         let shrunk := diskShrink bs_disk in
+         let replaced := match diskGet bs_disk n with
+                                               | None => block0
+                                               | Some a => a
+                                               end in
+         diskUpd shrunk bs_addr replaced
+        ).
+      intuition.
 
-  Theorem read_ok : forall a, proc_spec (OneDiskAPI.read_spec a) (read a) recover abstr.
-  Proof.
-    unfold read.
-    intros.
+      simpl.
 
-    apply spec_abstraction_compose; simpl.
-    step_proc; eauto.
+      constructor.
 
-    destruct (a == r).
-    - admit.
-    - admit.
-  Admitted.
+      {
+        intros.
+        destruct H0.
 
+        assert (a0 < diskSize (stateDisk state) - 1).
+        {
+          rewrite diskUpd_size in H0.
+          rewrite diskShrink_size in H0.
+          2: {
+            rewrite <- H1. lia.
+          }
+          assumption.
+        }
 
-  Theorem bad_block_inbounds :
+        rewrite <- diskShrink_preserves.
+        2: {
+          rewrite diskShrink_size.
+          2: {
+            rewrite <- H1. lia.
+          }
+          lia.
+        }
+
+        rewrite -> diskUpd_neq.
+        2: {
+          lia.
+        }
+        trivial.
+      }
+      {
+        intros.
+        rewrite diskUpd_size in H0.
+        rewrite diskShrink_size in H0.
+        2: {
+          rewrite <- H1. lia.
+        }
+
+        rewrite -> diskUpd_eq.
+        2: {
+          rewrite diskShrink_size.
+          2: {
+            rewrite <- H1. lia.
+          }
+          lia.
+        }
+        assert (n = diskSize (stateDisk state) - 1).
+        { lia. }
+
+        assert (forall (z : nat) (r : block) (d : disk), z < diskSize d -> Some (match diskGet d z with
+                                       | Some q => q
+                                       | None => r
+                                       end) = diskGet d z
+               ).
+        {
+          intros.
+          edestruct (diskGet d z) eqn:Heq.
+          {
+            trivial.
+          }
+          {
+            apply disk_inbounds_not_none in Heq.
+            2: { trivial. }
+            contradiction.
+          }
+        }
+        rewrite <- H2.
+        apply H3.
+        lia.
+      }
+      {
+        rewrite diskUpd_size.
+        rewrite diskShrink_size; lia.
+      }
+    }
+    {
+      step_proc.
+    }
+  Qed.
+
+Theorem bad_block_inbounds :
     forall state,
       stateBadBlock state < diskSize (stateDisk state).
   Proof.
@@ -143,37 +279,292 @@ Module RemappedDisk (bd : BadBlockAPI) <: OneDiskAPI.
     exact stateBadBlockInBounds.
   Qed.
 
-  Theorem remapped_abstraction_diskUpd_remap : forall state state' s v,
+
+
+  Theorem read_ok : forall a, proc_spec (OneDiskAPI.read_spec a) (read a) recover abstr.
+  Proof.
+    unfold read.
+    intros.
+
+    apply spec_abstraction_compose; simpl.
+    step_proc; eauto.
+
+    destruct (a == r) eqn:Heq1.
+    {
+
+      step_proc.
+      {
+       exists state2. intuition.
+      }
+      step_proc.
+      {
+        exists state2. intuition.
+      }
+      step_proc; intuition.
+      {
+        exists state2. intuition.
+        invert_abstraction.
+
+        destruct (diskSize (stateDisk state) - 1 == stateBadBlock state).
+        {
+          (* bad block is out of bounds of spec; so diskGet spec bad_block is none.
+           so any maybe_eq statement about it is true. *)
+          assert (diskGet state2 (stateBadBlock state) = None).
+          {
+            rewrite <- e.
+            rewrite -> Hsize.
+
+            rewrite -> disk_oob_eq.
+            2: {
+              lia.
+            }
+            trivial.
+          }
+          unfold maybe_eq.
+          apply holds_in_none_eq.
+          assumption.
+        }
+        {
+          (* bad block is not out of bounds. *)
+          rewrite <- Hbadblock in H2.
+          {
+            apply H2 in n.
+            assumption.
+          }
+
+          assert (stateBadBlock state < diskSize (stateDisk state)).
+          {
+            apply bad_block_inbounds.
+          }
+          lia.
+        }
+      }
+      {
+        exists state2. intuition.
+      }
+    }
+    step_proc.
+    {
+      exists state2. intuition.
+    }
+    step_proc.
+    {
+      exists state2. intuition.
+      invert_abstraction.
+      case (lt_dec a (diskSize state2)); intros.
+      {
+        rewrite <- Hgoodblocks.
+        2: {
+          intuition.
+        }
+        assumption.
+      }
+      {
+        assert (diskGet state2 a = None).
+        {
+          apply disk_oob_eq.
+          assumption.
+        }
+        unfold maybe_eq.
+        apply holds_in_none_eq.
+        assumption.
+      }
+    }
+    exists state2. intuition.
+  Qed.
+
+  (* Hint: you may find it useful to use the [pose proof (bad_block_inbounds state)]
+     if you need [lia] to make use of the fact that the bad block is in-bounds. *)
+
+  Theorem remapped_abstraction_diskUpd_remap : forall state state' s v_,
     remapped_abstraction state s ->
     stateBadBlock state' = stateBadBlock state ->
-    stateDisk state' = diskUpd (stateDisk state) (diskSize (stateDisk state) - 1) v ->
-    remapped_abstraction state' (diskUpd s (stateBadBlock state) v).
+    stateDisk state' = diskUpd (stateDisk state) (diskSize (stateDisk state) - 1) v_ ->
+    remapped_abstraction state' (diskUpd s (stateBadBlock state) v_).
   Proof.
-    (* Hint: you may find it useful to use the [pose proof (bad_block_inbounds state)]
-       if you need [lia] to make use of the fact that the bad block is in-bounds. *)
-    Admitted.
+    (*
+      given a state,
+      if we update the last slot,
+      that maps to updating the bad block in the spec.
+     *)
+    intros.
+    constructor.
+    {
+      (* proving Hgoodblocks. *)
+      intros. intuition.
+      invert_abstraction.
+      rewrite -> H0 in H3.
+      rewrite -> diskUpd_size in H2.
+      rewrite -> H1.
+      repeat rewrite -> diskUpd_neq by lia.
+      apply Hgoodblocks.
+      intuition.
+    }
+    {
+      (* proving Hbadblock. *)
+      intros.
+      rewrite -> H0.
+      rewrite -> H0 in H2.
+      rewrite -> diskUpd_size in H2.
+      rewrite -> H1.
+      rewrite -> diskUpd_size.
+      invert_abstraction.
+      repeat rewrite -> diskUpd_eq by lia.
+      trivial.
+    }
+    {
+      (* proving Hsize. *)
+      rewrite -> H1.
+      rewrite diskUpd_size.
+      rewrite diskUpd_size.
+      invert_abstraction.
+      assumption.
+    }
+  Qed.
 
 
-  Theorem remapped_abstraction_diskUpd_noremap : forall state state' s a v,
+  Theorem remapped_abstraction_diskUpd_noremap : forall state state' s a v_,
     remapped_abstraction state s ->
     a <> diskSize (stateDisk state) - 1 ->
     a <> stateBadBlock state ->
     stateBadBlock state' = stateBadBlock state ->
-    stateDisk state' = diskUpd (stateDisk state) a v ->
-    remapped_abstraction state' (diskUpd s a v).
+    stateDisk state' = diskUpd (stateDisk state) a v_ ->
+    remapped_abstraction state' (diskUpd s a v_).
   Proof.
-    Admitted.
+    (*
+      given a state, and an address that is neither the bad block
+      nor the final block, updating the address is equivalent to updating
+      the spec.
+     *)
+    intros. constructor.
+    {
+      (* Proving Hgoodblocks. *)
+      intros. intuition.
+      rewrite -> H2 in H5.
+      rewrite -> diskUpd_size in H4.
+      rewrite -> H3.
+      invert_abstraction.
+      case (equal_dec a a0).
+      {
+        intros.
+        rewrite <- e.
+        repeat rewrite diskUpd_eq by lia.
+        trivial.
+      }
+      {
+        intros.
+        repeat rewrite diskUpd_neq by lia.
+        apply Hgoodblocks.
+        lia.
+      }
+    }
+    {
+      (* Proving Hbadblock. *)
+      intros.
+      rewrite -> H2 in H4.
+      rewrite -> H2.
+      rewrite -> H3.
+      invert_abstraction.
+      rewrite -> diskUpd_size.
+      repeat rewrite diskUpd_neq by lia.
+      apply Hbadblock.
+      rewrite diskUpd_size in H4.
+      assumption.
+    }
+    {
+      (* Hsize. *)
+      rewrite -> H3.
+      rewrite diskUpd_size.
+      rewrite diskUpd_size.
+      invert_abstraction.
+      assumption.
+    }
+
+  Qed.
+
 
   Hint Resolve remapped_abstraction_diskUpd_remap : core.
   Hint Resolve remapped_abstraction_diskUpd_noremap : core.
 
-  Theorem write_ok : forall a v, proc_spec (OneDiskAPI.write_spec a v) (write a v) recover abstr.
+  Theorem write_ok : forall a v_, proc_spec (OneDiskAPI.write_spec a v_) (write a v_) recover abstr.
   Proof.
     unfold write.
     intros.
 
     apply spec_abstraction_compose; simpl.
-    Admitted.
+    step_proc.
+    {
+      exists state2. intuition.
+    }
+    case (equal_dec a r) as [Hwrite_bad | Hwrite_other].
+    {
+      step_proc.
+      {
+        exists state2. intuition.
+      }
+      step_proc.
+      {
+        destruct H1 as [Hcrash_before | Hcrash_after].
+        {
+          exists state2. intuition.
+        }
+        {
+          exists (diskUpd state2 (stateBadBlock state) v_). intuition.
+        }
+      }
+      step_proc.
+      {
+        exists (diskUpd state2 (stateBadBlock state) v_). intuition.
+      }
+      exists (diskUpd state2 (stateBadBlock state) v_). intuition.
+    }
+    {
+      step_proc.
+      {
+        exists state2. intuition.
+      }
+      case (equal_dec a (r - 1)) as [Hwrite_silly | Hwrite_nonsilly].
+      {
+        step_proc.
+        {
+          exists state2. intuition.
+          invert_abstraction.
+          rewrite Hsize.
+          rewrite diskUpd_none.
+          2: {
+            rewrite -> disk_oob_eq by lia.
+            trivial.
+          }
+          trivial.
+        }
+        {
+          exists state2. intuition.
+        }
+      }
+      {
+        step_proc.
+        {
+          destruct H1 as [Hcrash_before | Hcrash_after].
+          {
+           exists state2. intuition.
+          }
+          {
+            exists (diskUpd state2 a v_).
+            intuition.
+            eauto.
+          }
+        }
+        step_proc.
+        {
+          exists (diskUpd state2 a v_). intuition. eauto.
+        }
+        {
+          exists (diskUpd state2 a v_). intuition. eauto.
+        }
+      }
+    }
+  Qed.
+
 
   Theorem size_ok : proc_spec OneDiskAPI.size_spec size recover abstr.
   Proof.
@@ -183,7 +574,16 @@ Module RemappedDisk (bd : BadBlockAPI) <: OneDiskAPI.
     apply spec_abstraction_compose; simpl.
 
     step_proc; eauto.
-    Admitted.
+    step_proc.
+    {
+      exists state2. intuition.
+      invert_abstraction.
+      rewrite -> Hsize. lia.
+    }
+    {
+      exists state2. intuition.
+    }
+  Qed.
 
   (* This proof proves that recovery corresponds to no_wipe. *)
   Theorem recover_wipe : rec_wipe recover abstr no_wipe.
