src/Lab3/LogImpl.v
@@ -56,8 +56,8 @@ Hint Resolve addr_to_block_ok : core.
 Notation "d [ a |-> b ]" := (diskUpd d a b) (at level 8, left associativity).
 Notation "d [ a |=> bs ]" := (diskUpds d a bs) (at level 8, left associativity).
 
-Opaque diskGet.
 
+(* from https://sympa.inria.fr/sympa/arc/coq-club/2014-02/msg00157.html *)
 
 (** In this lab, you will likely be doing reasoning about
     the contents of various disk blocks.  The following
@@ -65,11 +65,28 @@ Opaque diskGet.
 Theorem diskGet_eq_values : forall d a b b',
     diskGet d a =?= b ->
     diskGet d a =?= b' ->
+    (* note: you need this condition because in the None case =?= always holds *)
     a < diskSize d ->
     b = b'.
 Proof.
-  (* Fill in your proof here. *)
-Admitted.
+  intros.
+
+  assert (diskGet d a = Some b).
+  {
+    destruct (diskGet d a) eqn:Heq.
+    {
+      apply holds_in_some in H.
+      simpl in H.
+      intuition.
+    }
+    {
+      apply disk_inbounds_not_none in H1. 2: assumption.
+      contradiction.
+    }
+  }
+  rewrite -> H2 in *.
+  intuition.
+Qed.
 
 (** We use the above theorem to implement the [eq_values]
     tactic.  [eq_values] can be used when you have hypotheses
@@ -91,24 +108,230 @@ Ltac eq_values :=
 
 Module Log (d : OneDiskAPI) <: LogAPI.
 
-  (** Fill in your implementation and proof here, replacing
-      the placeholder statements below with your own definitions
-      and theorems as appropriate.  Feel free to introduce helper
-      procedures and helper theorems to structure your implementation
-      and proof. *)
+  (** spec
 
-  Definition init : proc InitResult := Ret Initialized.
-  Definition get : proc (list block) := Ret nil.
-  Definition append (bs : list block) : proc bool := Ret true.
-  Definition reset : proc unit := Ret tt.
+    The log provides three operations: [get], [append], and [reset].
+    The [get] retrieves all of the blocks currently in the log.
+
+    [append] adds blocks to the log.  The [append] is the most interesting
+    part of the log, because [append] must be atomic with respect to crashes.
+    That means that, if the system crashes in the middle of an [append],
+    either all of the (APPENDED) blocks should be present (i.e., returned by [get]),
+    or none of them should be present.
+
+    [append] returns a boolean to indicate whether it succeeded
+    or not.  The intent is that [append] might fail if the log
+    has grown too big on disk, and there's no room for the new
+    blocks.
+
+    Finally, [reset] logically clears the log, removing all entries.  This
+    also must be crash-safe: if the system crashes in the middle of clearing
+    the log, either the log contents should still be there, or the log should
+    appear to be empty (according to [get]).
+ *)
+
+  (** disk guarantees (from OneDiskAPI)
+
+    no preconditions, any disk state is valid.
+
+    size_spec: size returns the correct value.
+    read_spec: read returns the correct value if the read is in-bounds.
+    write_spec:
+      post: the disk has been updated correctly.
+      recovered: either the write went through to the disk, or it didn't.
+ *)
+
+  (** useful definitions
+
+    Definition addr := nat.
+    Definition disk := list block
+
+    Axiom diskGet (d : disk) (a : addr) : option block.
+    Axiom diskSize (d : disk) : nat := length d.
+    Axiom diskUpd d (a: addr) b : disk.
+    Axiom diskGets (d : disk) (a : addr) (count : nat) : list (option block).
+    Axiom diskUpds (d : disk) (a : addr) (blocks : list block) : disk.
+
+    Specification A T R State: A specification with
+        ghost variables A,
+        return type T,
+        recovery type R,
+        state type State.
+    It has members:
+       pre: Prop,
+       post: T -> State -> Prop,
+       recovered: R -> State -> Prop.
+    It is constructed with a set of ghost variables and a starting state.
+ *)
+
+  (** hints
+      It seems like proving examples of your abstraction relation can be impossible because
+      diskGet is opaque and so it doesn't simplify, even on a disk which is an explicit list
+      of blocks. You can remove the line Opaque diskGet. to get around this problem (it was
+      jkintended to protect your proofs from unfolding the definition; feel free to add it
+      back after proving the examples, or don't use it if you don't run into issues.)
+
+      The examples in this lab will require that you start with an encoded block, but
+      there's no function from a number to a block encoding that number. You can work around
+      this by proving your examples for an arbitrary block that encodes some number, say
+      forall block_2, block_to_addr block_2 = 2 -> .... You also might want to use some
+      arbitrary data blocks b1, b2, etc in your examples rather than just combinations of
+      block0 and block1.
+
+      You code will need to use recursion, and therefore your proofs will use induction.
+      You saw some examples of this way back in lab 0, so I encourage you to go see
+      what you did there.
+   *)
+
+  (** implementation sketch
+
+    data layout:
+      last entry: log length
+      other entries: log elements
+   *)
+
+  (** helpers *)
+  Definition diskGetLogLength (d : disk) : nat :=
+    match diskGet d (diskSize d - 1) with
+    | Some v => block_to_addr v
+    | None => 0
+    end.
+
+  Example list_order : nth_error ([1; 2; 3]) 0 = Some 1.
+  Proof.
+    intuition.
+  Qed.
+
+
+  (** define the abstraction first, so we can interleave definitions and proofs *)
+
+  Inductive log_abstraction (disk_state : OneDiskAPI.State) (log_state : LogAPI.State) : Prop :=
+    (* fun fact: both states are just `list block` *)
+
+    | LogAbstraction :
+      let nonsense := 0 in
+      forall
+        (* maximum log length is (disk size - 1) *)
+        (Hlength_inbounds : length log_state < length disk_state)
+        (* last entry on disk is the same as log length (or log length is 0) *)
+        (Hlength_on_disk : length log_state = diskGetLogLength disk_state)
+        (* for all nats i below log length, the block at i on the disk corresponds to the block at i in the log. *)
+        (Hentries : forall i : nat, i < length log_state -> diskGet disk_state i = nth_error log_state i)
+      ,
+      log_abstraction disk_state log_state.
+  Definition abstr : Abstraction State :=
+    abstraction_compose d.abstr {| abstraction := log_abstraction |}.
+  Hint Constructors log_abstraction : core.
+
+  Example abstr_1_ok : forall (len2 : block), block_to_addr len2 = 2 ->
+log_abstraction ([block0; block1; len2]) ([block0; block1]).
+  Proof.
+    constructor; eauto; intros; simpl; simpl in *.
+    destruct (i == 0); intuition.
+    destruct (i == 1); intuition.
+    lia.
+  Qed.
+
+  Example abstr_2_ok : forall (len0 : block), block_to_addr len0 = 0 ->
+                                         log_abstraction ([block0; block0; len0]) ([]).
+  Proof.
+    constructor; eauto; intros; simpl; simpl in *; lia.
+  Qed.
+
+  Example abstr_3_ok : forall (len2 : block), block_to_addr len2 = 2 ->
+                                         log_abstraction ([block0; block1; block0; len2]) ([block0; block1]).
+  Proof.
+    constructor; eauto; intros; simpl; simpl in *.
+    {
+      lia.
+    }
+    destruct (i == 0); intuition.
+    destruct (i == 1); intuition.
+    lia.
+  Qed.
+
+
+  (* Recovery is a noop. *)
   Definition recover : proc unit := Ret tt.
-
-  Axiom abstr : Abstraction State.
-  Axiom init_ok : init_abstraction init recover abstr inited_any.
-  Axiom get_ok : proc_spec get_spec get recover abstr.
-  Axiom append_ok : forall v, proc_spec (append_spec v) (append v) recover abstr.
-  Axiom reset_ok : proc_spec reset_spec reset recover abstr.
   Axiom recover_wipe : rec_wipe recover abstr no_wipe.
+
+
+  (* Helper: get log length from disk. *)
+  Definition log_length : proc nat :=
+    sz <- d.size;
+    if gt_dec sz 0 then
+      len <- d.read (sz - 1);
+      Ret (block_to_addr len)
+    else
+      Ret 0.
+  Definition log_length_spec : Specification unit nat unit OneDiskAPI.State :=
+    fun (_ : unit) state => {|
+        pre := True;
+        post := fun r state' =>
+                 state' = state /\
+                 diskGetLogLength state = r;
+        recovered := fun _ state' =>
+                      state' = state
+      |}.
+  Axiom length_ok : proc_spec log_length_spec log_length recover abstr.
+
+
+  (* we don't prove anything about set_log_length; just handle it in proofs. *)
+  Definition set_log_length (n : nat): proc unit :=
+    sz <- d.size;
+    n_ <- addr_to_block n;
+    _ <- d.write (sz - 1) n_;
+    Ret tt.
+
+
+  (* to initialize, just set length to 0. *)
+  Definition init : proc InitResult :=
+    _ <- set_log_length 0;
+    Ret Initialized.
+  Axiom init_ok : init_abstraction init recover abstr inited_any.
+
+
+  (* helper for `get`. note: addr goes up as remaining goes down *)
+  Fixpoint get_rec (addr : nat) (remaining : nat) : proc (list block) :=
+    match remaining with
+    | 0 =>
+      Ret nil
+    | S remaining_ =>
+      b <- d.read addr;
+        rest <- get_rec (S addr) remaining_;
+        Ret (b :: rest)
+    end.
+  Definition get : proc (list block) :=
+    len <- log_length;
+    r <- get_rec 0 len;
+    Ret r.
+  Axiom get_ok : proc_spec get_spec get recover abstr.
+
+
+  (* helper for `get`. note: addr goes up as bs shrinks *)
+  Fixpoint append_rec (addr : nat) (bs : list block) : proc unit :=
+    match bs with
+    | nil =>
+      Ret tt
+    | cons b bs_ =>
+      _ <- d.write addr b;
+      _ <- append_rec (S addr) bs_;
+      Ret tt
+    end.
+  Definition append (bs : list block) : proc bool :=
+    size <- d.size;
+    len <- log_length;
+    if lt_dec (len + length bs) size then
+      _ <- append_rec len bs;
+      Ret true
+    else
+      Ret false.
+  Axiom append_ok : forall v, proc_spec (append_spec v) (append v) recover abstr.
+
+  Definition reset : proc unit :=
+    _ <- set_log_length 0;
+    Ret tt.
+  Axiom reset_ok : proc_spec reset_spec reset recover abstr.
 
 
 End Log.
